Add return values/postcondition to heaplang adequacy (modulo several admitted proofs).

src/heaplang/adequacy.v
@@ -84,16 +84,38 @@ Proof.
   destruct (to_val _) eqn:Heq; by simpl_itree.
 Qed.
 
-Definition compile_tp (tp : list expr) : list (itree heaplangE ()) :=
-  map (λ e, compile_expr e ;; yield_if_not_val e ;; kill_thread)%itree tp.
-
-Lemma compile_tp_app (tp tp' : list expr) :
-  compile_tp (tp ++ tp') = compile_tp tp ++ compile_tp tp'.
-Proof. rewrite /compile_tp map_app //. Qed.
+Definition compile_tp' (tp : list expr) : list (itree heaplangE val) :=
+  map (λ e,
+    compile_expr e ;;
+    yield_if_not_val e ;;
+    kill_thread
+  )%itree tp.
+Definition compile_tp (tp : list expr) : list (itree heaplangE val) :=
+  map (λ '(tid, e),
+    v ← compile_expr e ;
+    yield_if_not_val e ;;
+    match tid with
+    | 0 => Ret v
+    | _ => kill_thread
+    end
+  )%itree (enumerate tp).
 
 Lemma compile_tp_len tp :
   length (compile_tp tp) = length tp.
-Proof. rewrite /compile_tp map_length //. Qed.
+Proof. rewrite /compile_tp map_length enumerate_length //. Qed.
+Lemma compile_tp'_app tp tp' :
+  compile_tp' (tp ++ tp') = compile_tp' tp ++ compile_tp' tp'.
+Admitted.
+Lemma compile_tp'_cons e tp :
+  compile_tp' (e :: tp) = compile_tp' [e] ++ compile_tp' tp.
+Admitted.
+Lemma compile_tp_app tp tp' :
+  length tp ≠ 0 →
+  compile_tp (tp ++ tp') = compile_tp tp ++ compile_tp' tp'.
+Admitted.
+Lemma compile_tp_cons e tp :
+  compile_tp (e :: tp) = compile_tp [e] ++ compile_tp' tp.
+Admitted.
 
 Global Instance reducible_dec (e : expr) σ : Decision (reducible e σ).
 Admitted.
@@ -380,7 +402,7 @@ Proof.
   - exists [], (Resolve e1 e2 e3). split; first done. by split; first constructor.
 Qed.
 
-Lemma is_ctrace_ub tp tid (k : void → itree heaplangE ()) :
+Lemma is_ctrace_ub {R} tp tid (k : void → itree heaplangE R) :
   tp !! tid = Some (x ← trigger EUb ; k x)%itree →
   is_ctrace (CTVisEmpty void (subevent _ EUb)) tid tp.
 Proof.
@@ -397,9 +419,82 @@ Definition thread_stuck (tp : list expr) σ :=
 Global Instance thread_stuck_dec tp σ : Decision (thread_stuck tp σ).
 Admitted.
 
-Definition trace_invariant σ tp' σ' (tr : ctrace (demonicE +' stateE state +' ubE) ()) :=
-  (thread_stuck tp' σ' → is_postfix_ctrace (CTVisEmpty void (subevent _ EUb)) tr) ∧
+Variant Terminal (R : Type) :=
+  | TermRet (r : R)
+  | TermUb.
+Arguments TermRet {_}.
+Arguments TermUb {_}.
+Definition terminal_trace {E R} `{ubE -< E} (tx : Terminal R) : trace E R :=
+  match tx with
+  | TermRet r => TRet r
+  | TermUb => TVisEmpty void (subevent _ EUb)
+  end.
+Definition terminal_ctrace {E R} `{ubE -< E} (tx : Terminal R) : ctrace E R :=
+  match tx with
+  | TermRet r => CTRet r
+  | TermUb => CTVisEmpty void (subevent _ EUb)
+  end.
+
+Instance Terminal_FMap : FMap Terminal :=
+  λ _ _ f tx,
+    match tx with
+    | TermRet r => TermRet (f r)
+    | TermUb => TermUb
+    end.
+
+Definition trace_terminates_in {E R} `{ubE -< E} (tr : trace E R) (tx : Terminal R) :=
+  is_postfix (terminal_trace tx) tr.
+Definition ctrace_terminates_in {E R} `{ubE -< E} (tr : ctrace E R) (tx : Terminal R) :=
+  is_postfix_ctrace (terminal_ctrace tx) tr.
+
+Definition tp_termination (tp : list expr) (σ : state) : option (Terminal val) :=
+  match tp with
+  | (Val v)::_ => Some (TermRet v)
+  | _ => if decide (thread_stuck tp σ) then Some TermUb else None
+  end.
+
+Definition trace_invariant_postfix tp' σ' (tr : ctrace (demonicE +' stateE state +' ubE) val) :=
+  match tp_termination tp' σ' with
+  | Some tx => ctrace_terminates_in tr tx
+  | None => False
+  end.
+Definition trace_invariant σ tp' σ' (tr : ctrace (demonicE +' stateE state +' ubE) val) :=
+  trace_invariant_postfix tp' σ' tr ∧
   is_Some (interp_tr_state σ (interp_tr (sequencify tr))).
+
+Definition undone_tp (tp : list expr) :=
+  ∃ e_fst,
+  tp !! 0 = Some e_fst ∧
+  to_val e_fst = None.
+
+Lemma done_or_undone tp :
+  (∃ v, tp !! 0 = Some (Val v)) ∨ undone_tp tp.
+Admitted.
+
+Lemma trace_invariant_postfix_undone tp' σ' tr :
+  undone_tp tp' →
+  (thread_stuck tp' σ' → is_postfix_ctrace (CTVisEmpty void (subevent _ EUb)) tr) →
+  trace_invariant_postfix tp' σ' tr.
+Admitted.
+
+Lemma trace_invariant_postfix_postfix tp' σ' tr tr' :
+  is_postfix_ctrace tr tr' →
+  trace_invariant_postfix tp' σ' tr →
+  trace_invariant_postfix tp' σ' tr'.
+Proof.
+  intros Hpost Htinv. rewrite /trace_invariant_postfix. rewrite /trace_invariant_postfix in Htinv.
+  destruct tp'.
+Admitted.
+
+Lemma is_ctrace_done tp v :
+  tp !! 0 = Some (Val v) →
+  is_ctrace (CTRet v) 0 (compile_tp tp).
+Admitted.
+
+Lemma trace_invariant_done tp σ v :
+  tp !! 0 = Some (Val v) →
+  trace_invariant σ tp σ (CTRet v).
+Admitted.
 
 Lemma UnOp_stuck op v σ :
   stuck (UnOp op (Val v)) σ →
@@ -423,17 +518,24 @@ Proof.
   by constructor.
 Qed.
 
+Lemma enumerate_lookup' {A} (xs : list A) (tid : nat) :
+  (enumerate xs) !! tid = (λ x, (tid, x)) <$> (xs !! tid).
+Admitted.
+
 Lemma stuck_ub tp tid e σ :
   tp !! tid = Some e →
+  undone_tp tp →
   stuck e σ →
   ∃ tr, trace_invariant σ tp σ tr ∧ is_ctrace tr tid (compile_tp tp).
 Proof.
-  intros Htp (K&e'&->&Hbasic&Hstuck)%stuck_basic.
+  intros Htp Hundone (K&e'&->&Hbasic&Hstuck)%stuck_basic.
   destruct Hbasic as [x|f x e0|v1 v2 | | | | | | | | | | | | | | | | | | ].
   - exists (CTVisEmpty void (subevent _ EUb)).
-    split; first split; eauto. { intros _. constructor. }
+    split; first split.
+    { eapply trace_invariant_postfix_undone; eauto. intros Hstuck'. constructor. }
+    { done. }
     eapply is_ctrace_insert.
-    { rewrite /compile_tp list_lookup_fmap Htp //. }
+    { rewrite /compile_tp list_lookup_fmap enumerate_lookup' Htp //. }
     { rewrite compile_expr_bind'; first done. admit. }
     rewrite /compile_expr. simpl_itree.
     eapply is_ctrace_ub.
@@ -442,9 +544,10 @@ Proof.
     eapply Ectx_step with (K := []); eauto.
     by constructor.
   - exists (CTVisEmpty void (subevent _ EUb)).
-    split; first split; eauto. { intros _. constructor. }
+    split; first split; eauto.
+    { eapply trace_invariant_postfix_undone; eauto. intros Hstuck'. constructor. }
     eapply is_ctrace_insert.
-    { rewrite /compile_tp list_lookup_fmap Htp //. }
+    { rewrite /compile_tp list_lookup_fmap enumerate_lookup' Htp //. }
     { rewrite compile_expr_bind'; first done. admit. }
     destruct (val_to_RecV v1) as [[[f x] e]|] eqn:Heq.
     * destruct v1; try discriminate.
@@ -455,27 +558,30 @@ Proof.
       eapply is_ctrace_ub.
       rewrite list_lookup_insert // compile_tp_len -lookup_lt_is_Some //.
   - exists (CTVisEmpty void (subevent _ EUb)).
-    split; first split; eauto. { intros _. constructor. }
+    split; first split; eauto.
+    { eapply trace_invariant_postfix_undone; eauto. intros Hstuck'. constructor. }
     eapply is_ctrace_insert.
-    { rewrite /compile_tp list_lookup_fmap Htp //. }
+    { rewrite /compile_tp list_lookup_fmap enumerate_lookup' Htp //. }
     { rewrite compile_expr_bind'; first done. admit. }
     rewrite /compile_expr. simpl_itree.
     apply UnOp_stuck in Hstuck as ->.
     simpl_itree. eapply is_ctrace_ub.
     rewrite list_lookup_insert // compile_tp_len -lookup_lt_is_Some //.
   - exists (CTVisEmpty void (subevent _ EUb)).
-    split; first split; eauto. { intros _. constructor. }
+    split; first split; eauto.
+    { eapply trace_invariant_postfix_undone; eauto. intros Hstuck'. constructor. }
     eapply is_ctrace_insert.
-    { rewrite /compile_tp list_lookup_fmap Htp //. }
+    { rewrite /compile_tp list_lookup_fmap enumerate_lookup' Htp //. }
     { rewrite compile_expr_bind'; first done. admit. }
     rewrite /compile_expr. simpl_itree.
     apply BinOp_stuck in Hstuck as ->.
     simpl_itree. eapply is_ctrace_ub.
     rewrite list_lookup_insert // compile_tp_len -lookup_lt_is_Some //.
   - exists (CTVisEmpty void (subevent _ EUb)).
-    split; first split; eauto. { intros _. constructor. }
+    split; first split; eauto.
+    { eapply trace_invariant_postfix_undone; eauto. intros Hstuck'. constructor. }
     eapply is_ctrace_insert.
-    { rewrite /compile_tp list_lookup_fmap Htp //. }
+    { rewrite /compile_tp list_lookup_fmap enumerate_lookup' Htp //. }
     { rewrite compile_expr_bind'; first done. admit. }
     destruct (val_to_bool v0) as [|] eqn:Heq.
     * destruct v0; try discriminate. destruct l; try discriminate.
@@ -490,9 +596,10 @@ Proof.
     eapply Ectx_step with (K := []); eauto.
     by constructor.
   - exists (CTVisEmpty void (subevent _ EUb)).
-    split; first split; eauto. { intros _. constructor. }
+    split; first split; eauto.
+    { eapply trace_invariant_postfix_undone; eauto. intros Hstuck'. constructor. }
     eapply is_ctrace_insert.
-    { rewrite /compile_tp list_lookup_fmap Htp //. }
+    { rewrite /compile_tp list_lookup_fmap enumerate_lookup' Htp //. }
     { rewrite compile_expr_bind'; first done. admit. }
     destruct (val_to_pair v) as [[x y]|] eqn:Heq.
     * destruct v; try discriminate.
@@ -503,9 +610,10 @@ Proof.
       eapply is_ctrace_ub.
       rewrite list_lookup_insert // compile_tp_len -lookup_lt_is_Some //.
   - exists (CTVisEmpty void (subevent _ EUb)).
-    split; first split; eauto. { intros _. constructor. }
+    split; first split; eauto.
+    { eapply trace_invariant_postfix_undone; eauto. intros Hstuck'. constructor. }
     eapply is_ctrace_insert.
-    { rewrite /compile_tp list_lookup_fmap Htp //. }
+    { rewrite /compile_tp list_lookup_fmap enumerate_lookup' Htp //. }
     { rewrite compile_expr_bind'; first done. admit. }
     destruct (val_to_pair v) as [[x y]|] eqn:Heq.
     * destruct v; try discriminate.
@@ -522,9 +630,10 @@ Proof.
     eapply Ectx_step with (K := []); eauto.
     by constructor.
   - exists (CTVisEmpty void (subevent _ EUb)).
-    split; first split; eauto. { intros _. repeat constructor. }
+    split; first split; eauto.
+    { eapply trace_invariant_postfix_undone; eauto. intros Hstuck'. constructor. }
     eapply is_ctrace_insert.
-    { rewrite /compile_tp list_lookup_fmap Htp //. }
+    { rewrite /compile_tp list_lookup_fmap enumerate_lookup' Htp //. }
     { rewrite compile_expr_bind'; first done. admit. }
     destruct (val_to_sum v0) as [[x|y]|] eqn:Heq.
     * destruct v0; try discriminate.
@@ -542,9 +651,10 @@ Proof.
     eapply Ectx_step with (K := []); eauto.
     by constructor.
   - exists (CTVisEmpty void (subevent _ EUb)).
-    split; first split; eauto. { intros _. constructor. }
+    split; first split; eauto.
+    { eapply trace_invariant_postfix_undone; eauto. intros Hstuck'. constructor. }
     eapply is_ctrace_insert.
-    { rewrite /compile_tp list_lookup_fmap Htp //. }
+    { rewrite /compile_tp list_lookup_fmap enumerate_lookup' Htp //. }
     { rewrite compile_expr_bind'; first done. admit. }
     destruct (val_to_int nv) as [n|] eqn:Heq.
     * destruct nv; try discriminate. destruct l; try discriminate.
@@ -570,10 +680,10 @@ Proof.
         by eapply FreeS.
       + exists (CTVis state (subevent _ EGetState) σ (CTVisEmpty void (subevent _ EUb))).
         split; first split.
-        ++ intros _. repeat constructor.
+        ++ eapply trace_invariant_postfix_undone; eauto. intros Hstuck'. repeat constructor.
         ++ simpl. rewrite decide_True //.
         ++ eapply is_ctrace_insert.
-           { rewrite /compile_tp list_lookup_fmap Htp //. }
+           { rewrite /compile_tp list_lookup_fmap enumerate_lookup' Htp //. }
            { rewrite compile_expr_bind'; first done. admit. }
            rewrite /compile_expr. simpl_itree. rewrite Heq /=. simpl_itree.
            eapply is_ctrace_Vis.
@@ -583,10 +693,10 @@ Proof.
            rewrite list_lookup_insert // insert_length compile_tp_len -lookup_lt_is_Some //.
       + exists (CTVis state (subevent _ EGetState) σ (CTVisEmpty void (subevent _ EUb))).
         split; first split.
-        ++ intros _. repeat constructor.
+        ++ eapply trace_invariant_postfix_undone; eauto. intros Hstuck'. repeat constructor.
         ++ simpl. rewrite decide_True //.
         ++ eapply is_ctrace_insert.
-           { rewrite /compile_tp list_lookup_fmap Htp //. }
+           { rewrite /compile_tp list_lookup_fmap enumerate_lookup' Htp //. }
            { rewrite compile_expr_bind'; first done. admit. }
            rewrite /compile_expr. simpl_itree. rewrite Heq /=. simpl_itree.
            eapply is_ctrace_Vis.
@@ -595,9 +705,10 @@ Proof.
            eapply is_ctrace_ub.
            rewrite list_lookup_insert // insert_length compile_tp_len -lookup_lt_is_Some //.
     * exists (CTVisEmpty void (subevent _ EUb)).
-      split; first split; eauto. { intros _. constructor. }
+      split; first split; eauto.
+      { eapply trace_invariant_postfix_undone; eauto. intros Hstuck'. constructor. }
       eapply is_ctrace_insert.
-      { rewrite /compile_tp list_lookup_fmap Htp //. }
+      { rewrite /compile_tp list_lookup_fmap enumerate_lookup' Htp //. }
       { rewrite compile_expr_bind'; first done. admit. }
       rewrite /compile_expr. simpl_itree. rewrite Heq /=. simpl_itree.
       eapply is_ctrace_ub.
@@ -612,10 +723,10 @@ Proof.
         by eapply LoadS.
       + exists (CTVis state (subevent _ EGetState) σ (CTVisEmpty void (subevent _ EUb))).
         split; first split.
-        ++ intros _. repeat constructor.
+        ++ eapply trace_invariant_postfix_undone; eauto. intros Hstuck'. repeat constructor.
         ++ simpl. rewrite decide_True //.
         ++ eapply is_ctrace_insert.
-           { rewrite /compile_tp list_lookup_fmap Htp //. }
+           { rewrite /compile_tp list_lookup_fmap enumerate_lookup' Htp //. }
            { rewrite compile_expr_bind'; first done. admit. }
            rewrite /compile_expr. simpl_itree. rewrite Heq /=. simpl_itree.
            eapply is_ctrace_Vis.
@@ -625,10 +736,10 @@ Proof.
            rewrite list_lookup_insert // insert_length compile_tp_len -lookup_lt_is_Some //.
       + exists (CTVis state (subevent _ EGetState) σ (CTVisEmpty void (subevent _ EUb))).
         split; first split.
-        ++ intros _. repeat constructor.
+        ++ eapply trace_invariant_postfix_undone; eauto. intros Hstuck'. repeat constructor.
         ++ simpl. rewrite decide_True //.
         ++ eapply is_ctrace_insert.
-           { rewrite /compile_tp list_lookup_fmap Htp //. }
+           { rewrite /compile_tp list_lookup_fmap enumerate_lookup' Htp //. }
            { rewrite compile_expr_bind'; first done. admit. }
            rewrite /compile_expr. simpl_itree. rewrite Heq /=. simpl_itree.
            eapply is_ctrace_Vis.
@@ -637,9 +748,10 @@ Proof.
            eapply is_ctrace_ub.
            rewrite list_lookup_insert // insert_length compile_tp_len -lookup_lt_is_Some //.
     * exists (CTVisEmpty void (subevent _ EUb)).
-      split; first split; eauto. { intros _. constructor. }
+      split; first split; eauto.
+      { eapply trace_invariant_postfix_undone; eauto. intros Hstuck'. constructor. }
       eapply is_ctrace_insert.
-      { rewrite /compile_tp list_lookup_fmap Htp //. }
+      { rewrite /compile_tp list_lookup_fmap enumerate_lookup' Htp //. }
       { rewrite compile_expr_bind'; first done. admit. }
       rewrite /compile_expr. simpl_itree. rewrite Heq /=. simpl_itree.
       eapply is_ctrace_ub.
@@ -654,10 +766,10 @@ Proof.
         by eapply StoreS.
       + exists (CTVis state (subevent _ EGetState) σ (CTVisEmpty void (subevent _ EUb))).
         split; first split.
-        ++ intros _. repeat constructor.
+        ++ eapply trace_invariant_postfix_undone; eauto. intros Hstuck'. repeat constructor.
         ++ simpl. rewrite decide_True //.
         ++ eapply is_ctrace_insert.
-           { rewrite /compile_tp list_lookup_fmap Htp //. }
+           { rewrite /compile_tp list_lookup_fmap enumerate_lookup' Htp //. }
            { rewrite compile_expr_bind'; first done. admit. }
            rewrite /compile_expr. simpl_itree. rewrite Heq /=. simpl_itree.
            eapply is_ctrace_Vis.
@@ -667,10 +779,10 @@ Proof.
            rewrite list_lookup_insert // insert_length compile_tp_len -lookup_lt_is_Some //.
       + exists (CTVis state (subevent _ EGetState) σ (CTVisEmpty void (subevent _ EUb))).
         split; first split.
-        ++ intros _. repeat constructor.
+        ++ eapply trace_invariant_postfix_undone; eauto. intros Hstuck'. repeat constructor.
         ++ simpl. rewrite decide_True //.
         ++ eapply is_ctrace_insert.
-           { rewrite /compile_tp list_lookup_fmap Htp //. }
+           { rewrite /compile_tp list_lookup_fmap enumerate_lookup' Htp //. }
            { rewrite compile_expr_bind'; first done. admit. }
            rewrite /compile_expr. simpl_itree. rewrite Heq /=. simpl_itree.
            eapply is_ctrace_Vis.
@@ -679,9 +791,10 @@ Proof.
            eapply is_ctrace_ub.
            rewrite list_lookup_insert // insert_length compile_tp_len -lookup_lt_is_Some //.
     * exists (CTVisEmpty void (subevent _ EUb)).
-      split; first split; eauto. { intros _. constructor. }
+      split; first split; eauto.
+      { eapply trace_invariant_postfix_undone; eauto. intros Hstuck'. constructor. }
       eapply is_ctrace_insert.
-      { rewrite /compile_tp list_lookup_fmap Htp //. }
+      { rewrite /compile_tp list_lookup_fmap enumerate_lookup' Htp //. }
       { rewrite compile_expr_bind'; first done. admit. }
       rewrite /compile_expr. simpl_itree. rewrite Heq /=. simpl_itree.
       eapply is_ctrace_ub.
@@ -696,10 +809,10 @@ Proof.
         by eapply XchgS.
       + exists (CTVis state (subevent _ EGetState) σ (CTVisEmpty void (subevent _ EUb))).
         split; first split.
-        ++ intros _. repeat constructor.
+        ++ eapply trace_invariant_postfix_undone; eauto. intros Hstuck'. repeat constructor.
         ++ simpl. rewrite decide_True //.
         ++ eapply is_ctrace_insert.
-           { rewrite /compile_tp list_lookup_fmap Htp //. }
+           { rewrite /compile_tp list_lookup_fmap enumerate_lookup' Htp //. }
            { rewrite compile_expr_bind'; first done. admit. }
            rewrite /compile_expr. simpl_itree. rewrite Heq /=. simpl_itree.
            eapply is_ctrace_Vis.
@@ -709,10 +822,10 @@ Proof.
            rewrite list_lookup_insert // insert_length compile_tp_len -lookup_lt_is_Some //.
       + exists (CTVis state (subevent _ EGetState) σ (CTVisEmpty void (subevent _ EUb))).
         split; first split.
-        ++ intros _. repeat constructor.
+        ++ eapply trace_invariant_postfix_undone; eauto. intros Hstuck'. repeat constructor.
         ++ simpl. rewrite decide_True //.
         ++ eapply is_ctrace_insert.
-           { rewrite /compile_tp list_lookup_fmap Htp //. }
+           { rewrite /compile_tp list_lookup_fmap enumerate_lookup' Htp //. }
            { rewrite compile_expr_bind'; first done. admit. }
            rewrite /compile_expr. simpl_itree. rewrite Heq /=. simpl_itree.
            eapply is_ctrace_Vis.
@@ -721,9 +834,10 @@ Proof.
            eapply is_ctrace_ub.
            rewrite list_lookup_insert // insert_length compile_tp_len -lookup_lt_is_Some //.
     * exists (CTVisEmpty void (subevent _ EUb)).
-      split; first split; eauto. { intros _. constructor. }
+      split; first split; eauto.
+      { eapply trace_invariant_postfix_undone; eauto. intros Hstuck'. constructor. }
       eapply is_ctrace_insert.
-      { rewrite /compile_tp list_lookup_fmap Htp //. }
+      { rewrite /compile_tp list_lookup_fmap enumerate_lookup' Htp //. }
       { rewrite compile_expr_bind'; first done. admit. }
       rewrite /compile_expr. simpl_itree. rewrite Heq /=. simpl_itree.
       eapply is_ctrace_ub.
@@ -739,10 +853,10 @@ Proof.
            by eapply CmpXchgS.
         ++ exists (CTVis state (subevent _ EGetState) σ (CTVisEmpty void (subevent _ EUb))).
            split; first split.
-           +++ intros _. repeat constructor.
+           +++ eapply trace_invariant_postfix_undone; eauto. intros Hstuck'. repeat constructor.
            +++ simpl. rewrite decide_True //.
            +++ eapply is_ctrace_insert.
-               { rewrite /compile_tp list_lookup_fmap Htp //. }
+               { rewrite /compile_tp list_lookup_fmap enumerate_lookup' Htp //. }
                { rewrite compile_expr_bind'; first done. admit. }
                rewrite /compile_expr. simpl_itree. rewrite Heq /=. simpl_itree.
                eapply is_ctrace_Vis.
@@ -752,10 +866,10 @@ Proof.
                rewrite list_lookup_insert // insert_length compile_tp_len -lookup_lt_is_Some //.
       + exists (CTVis state (subevent _ EGetState) σ (CTVisEmpty void (subevent _ EUb))).
         split; first split.
-        ++ intros _. repeat constructor.
+        ++ eapply trace_invariant_postfix_undone; eauto. intros Hstuck'. repeat constructor.
         ++ simpl. rewrite decide_True //.
         ++ eapply is_ctrace_insert.
-           { rewrite /compile_tp list_lookup_fmap Htp //. }
+           { rewrite /compile_tp list_lookup_fmap enumerate_lookup' Htp //. }
            { rewrite compile_expr_bind'; first done. admit. }
            rewrite /compile_expr. simpl_itree. rewrite Heq /=. simpl_itree.
            eapply is_ctrace_Vis.
@@ -765,10 +879,10 @@ Proof.
            rewrite list_lookup_insert // insert_length compile_tp_len -lookup_lt_is_Some //.
       + exists (CTVis state (subevent _ EGetState) σ (CTVisEmpty void (subevent _ EUb))).
         split; first split.
-        ++ intros _. repeat constructor.
+        ++ eapply trace_invariant_postfix_undone; eauto. intros Hstuck'. repeat constructor.
         ++ simpl. rewrite decide_True //.
         ++ eapply is_ctrace_insert.
-           { rewrite /compile_tp list_lookup_fmap Htp //. }
+           { rewrite /compile_tp list_lookup_fmap enumerate_lookup' Htp //. }
            { rewrite compile_expr_bind'; first done. admit. }
            rewrite /compile_expr. simpl_itree. rewrite Heq /=. simpl_itree.
            eapply is_ctrace_Vis.
@@ -777,9 +891,10 @@ Proof.
            eapply is_ctrace_ub.
            rewrite list_lookup_insert // insert_length compile_tp_len -lookup_lt_is_Some //.
     * exists (CTVisEmpty void (subevent _ EUb)).
-      split; first split; eauto. { intros _. constructor. }
+      split; first split; eauto.
+      { eapply trace_invariant_postfix_undone; eauto. intros Hstuck'. constructor. }
       eapply is_ctrace_insert.
-      { rewrite /compile_tp list_lookup_fmap Htp //. }
+      { rewrite /compile_tp list_lookup_fmap enumerate_lookup' Htp //. }
       { rewrite compile_expr_bind'; first done. admit. }
       rewrite /compile_expr. simpl_itree. rewrite Heq /=. simpl_itree.
       eapply is_ctrace_ub.
@@ -800,10 +915,10 @@ Proof.
                by eapply FaaS.
            +++ exists (CTVis state (subevent _ EGetState) σ (CTVisEmpty void (subevent _ EUb))).
                split; first split.
-               ++++ intros _. repeat constructor.
+               ++++ eapply trace_invariant_postfix_undone; eauto. intros Hstuck'. repeat constructor.
                ++++ simpl. rewrite decide_True //.
                ++++ eapply is_ctrace_insert.
-                    { rewrite /compile_tp list_lookup_fmap Htp //. }
+                    { rewrite /compile_tp list_lookup_fmap enumerate_lookup' Htp //. }
                     { rewrite compile_expr_bind'; first done. admit. }
                     rewrite /compile_expr. simpl_itree. rewrite Heq Heq' /=. simpl_itree.
                     eapply is_ctrace_Vis.
@@ -813,10 +928,10 @@ Proof.
                     rewrite list_lookup_insert // insert_length compile_tp_len -lookup_lt_is_Some //.
         ++ exists (CTVis state (subevent _ EGetState) σ (CTVisEmpty void (subevent _ EUb))).
            split; first split.
-           +++ intros _. repeat constructor.
+           +++ eapply trace_invariant_postfix_undone; eauto. intros Hstuck'. repeat constructor.
            +++ simpl. rewrite decide_True //.
            +++ eapply is_ctrace_insert.
-               { rewrite /compile_tp list_lookup_fmap Htp //. }
+               { rewrite /compile_tp list_lookup_fmap enumerate_lookup' Htp //. }
                { rewrite compile_expr_bind'; first done. admit. }
                rewrite /compile_expr. simpl_itree. rewrite Heq Heq' /=. simpl_itree.
                eapply is_ctrace_Vis.
@@ -826,10 +941,10 @@ Proof.
                rewrite list_lookup_insert // insert_length compile_tp_len -lookup_lt_is_Some //.
         ++ exists (CTVis state (subevent _ EGetState) σ (CTVisEmpty void (subevent _ EUb))).
            split; first split.
-           +++ intros _. repeat constructor.
+           +++ eapply trace_invariant_postfix_undone; eauto. intros Hstuck'. repeat constructor.
            +++ simpl. rewrite decide_True //.
            +++ eapply is_ctrace_insert.
-               { rewrite /compile_tp list_lookup_fmap Htp //. }
+               { rewrite /compile_tp list_lookup_fmap enumerate_lookup' Htp //. }
                { rewrite compile_expr_bind'; first done. admit. }
                rewrite /compile_expr. simpl_itree. rewrite Heq Heq' /=. simpl_itree.
                eapply is_ctrace_Vis.
@@ -838,17 +953,19 @@ Proof.
                eapply is_ctrace_ub.
                rewrite list_lookup_insert // insert_length compile_tp_len -lookup_lt_is_Some //.
       + exists (CTVisEmpty void (subevent _ EUb)).
-        split; first split; eauto. { intros _. constructor. }
+        split; first split; eauto.
+        { eapply trace_invariant_postfix_undone; eauto. intros Hstuck'. constructor. }
         eapply is_ctrace_insert.
-        { rewrite /compile_tp list_lookup_fmap Htp //. }
+        { rewrite /compile_tp list_lookup_fmap enumerate_lookup' Htp //. }
         { rewrite compile_expr_bind'; first done. admit. }
         rewrite /compile_expr. simpl_itree. rewrite Heq Heq' /=. simpl_itree.
         eapply is_ctrace_ub.
         rewrite list_lookup_insert // compile_tp_len -lookup_lt_is_Some //.
     * exists (CTVisEmpty void (subevent _ EUb)).
-      split; first split; eauto. { intros _. constructor. }
+      split; first split; eauto.
+      { eapply trace_invariant_postfix_undone; eauto. intros Hstuck'. constructor. }
       eapply is_ctrace_insert.
-      { rewrite /compile_tp list_lookup_fmap Htp //. }
+      { rewrite /compile_tp list_lookup_fmap enumerate_lookup' Htp //. }
       { rewrite compile_expr_bind'; first done. admit. }
       rewrite /compile_expr. simpl_itree. rewrite Heq' /=. simpl_itree.
       eapply is_ctrace_ub.
@@ -864,10 +981,10 @@ Lemma AllocN_free_locations n v σ ρs l efs :
   ∃ (l' : free_locations n σ), `l' = l.
 Proof. intros Hbase. by exists (to_free_location n v σ ρs l efs Hbase). Qed.
 
-Lemma step_in_thread e1 σ1 κs e2 σ2 efs tr tid tid' tp (k : val → itree heaplangE ()) tp' σ' :
+Lemma step_in_thread e1 σ1 κs e2 σ2 efs tr tid tid' tp (k : val → itree heaplangE val) tp' σ' :
   base_step e1 σ1 κs e2 σ2 efs →
   is_ctrace tr tid' (<[tid:=(v ← compile_expr e2 ; yield_if_not_val e2 ;; k v)%itree]>tp
-                    ++ compile_tp efs) →
+                    ++ compile_tp' efs) →
   trace_invariant σ2 tp' σ' tr →
   tp !! tid = Some (v ← compile_expr e1 ; yield_if_not_val e1 ;; k v)%itree →
   ∃ tr', trace_invariant σ1 tp' σ' tr' ∧ is_ctrace tr' tid tp.
@@ -875,7 +992,7 @@ Proof.
   intros Hbase Htr [Hub Hstinv] Htp.
   inversion Hbase; subst; simpl in Htr; rewrite ?app_nil_r in Htr.
   - exists (CTYield tid' tr). split; first split; eauto.
-    { intros Hstuck. constructor. by apply Hub. }
+    { apply trace_invariant_postfix_postfix with (tr := tr); eauto. repeat constructor. }
     eapply is_ctrace_insert; first done.
     { simpl. rewrite /compile_expr. simpl_itree. reflexivity. }
     apply is_ctrace_yield with (t := k (RecV f x e)).
@@ -883,7 +1000,7 @@ Proof.
     rewrite list_insert_insert.
     by simpl_itree in Htr.
   - exists (CTYield tid' tr). split; first split; eauto.
-    { intros Hstuck. constructor. by apply Hub. }
+    { apply trace_invariant_postfix_postfix with (tr := tr); eauto. repeat constructor. }
     eapply is_ctrace_insert; first done.
     { simpl. rewrite /compile_expr. simpl_itree. reflexivity. }
     apply is_ctrace_yield with (t := k (PairV v1 v2)).
@@ -891,7 +1008,7 @@ Proof.
     rewrite list_insert_insert.
     by simpl_itree in Htr.
   - exists (CTYield tid' tr). split; first split; eauto.
-    { intros Hstuck. constructor. by apply Hub. }
+    { apply trace_invariant_postfix_postfix with (tr := tr); eauto. repeat constructor. }
     eapply is_ctrace_insert; first done.
     { simpl. rewrite /compile_expr. simpl_itree. reflexivity. }
     apply is_ctrace_yield with (t := k (InjLV v)).
@@ -899,7 +1016,7 @@ Proof.
     rewrite list_insert_insert.
     by simpl_itree in Htr.
   - exists (CTYield tid' tr). split; first split; eauto.
-    { intros Hstuck. constructor. by apply Hub. }
+    { apply trace_invariant_postfix_postfix with (tr := tr); eauto. repeat constructor. }
     eapply is_ctrace_insert; first done.
     { simpl. rewrite /compile_expr. simpl_itree. reflexivity. }
     apply is_ctrace_yield with (t := k (InjRV v)).
@@ -908,7 +1025,7 @@ Proof.
     by simpl_itree in Htr.
   - pose (e' := subst' x v2 (subst' f (RecV f x e0) e0)).
     exists (CTYield tid' tr). split; first split; eauto.
-    { intros Hstuck. constructor. by apply Hub. }
+    { apply trace_invariant_postfix_postfix with (tr := tr); eauto. repeat constructor. }
     destruct (to_val e') as [v|] eqn:Hval.
     * eapply is_ctrace_insert; first done.
       { simpl. rewrite base_Beta. simpl.
@@ -931,21 +1048,21 @@ Proof.
       { rewrite list_lookup_insert //. by apply lookup_lt_is_Some. }
       by rewrite list_insert_insert.
   - exists (CTYield tid' tr). split; first split; eauto.
-    { intros Hstuck. constructor. by apply Hub. }
+    { apply trace_invariant_postfix_postfix with (tr := tr); eauto. repeat constructor. }
     rewrite compile_expr_val !bind_ret_l in Htr.
     eapply is_ctrace_insert with (t' := (trigger EYield ;; k v')%itree); first done.
     { rewrite base_UnOp // bind_ret_l  //. }
     eapply is_ctrace_yield. { rewrite list_lookup_insert //. by apply lookup_lt_is_Some. }
     by rewrite list_insert_insert.
   - exists (CTYield tid' tr). split; first split; eauto.
-    { intros Hstuck. constructor. by apply Hub. }
+    { apply trace_invariant_postfix_postfix with (tr := tr); eauto. repeat constructor. }
     rewrite compile_expr_val !bind_ret_l in Htr.
     eapply is_ctrace_insert with (t' := (trigger EYield ;; k v')%itree); first done.
     { rewrite base_BinOp // bind_ret_l  //. }
     eapply is_ctrace_yield. { rewrite list_lookup_insert //. by apply lookup_lt_is_Some. }
     by rewrite list_insert_insert.
   - exists (CTYield tid' tr). split; first split; eauto.
-    { intros Hstuck. constructor. by apply Hub. }
+    { apply trace_invariant_postfix_postfix with (tr := tr); eauto. repeat constructor. }
     destruct (to_val e2) eqn:Hval.
     * apply of_to_val in Hval as <-.
       eapply is_ctrace_insert; first done.
@@ -963,7 +1080,7 @@ Proof.
       rewrite list_insert_insert.
       by simpl_itree in Htr.
   - exists (CTYield tid' tr). split; first split; eauto.
-    { intros Hstuck. constructor. by apply Hub. }
+    { apply trace_invariant_postfix_postfix with (tr := tr); eauto. repeat constructor. }
     destruct (to_val e2) eqn:Hval.
     * apply of_to_val in Hval as <-.
       eapply is_ctrace_insert; first done.
@@ -981,21 +1098,21 @@ Proof.
       rewrite list_insert_insert.
       by simpl_itree in Htr.
   - exists (CTYield tid' tr). split; first split; eauto.
-    { intros Hstuck. constructor. by apply Hub. }
+    { apply trace_invariant_postfix_postfix with (tr := tr); eauto. repeat constructor. }
     rewrite compile_expr_val !bind_ret_l in Htr.
     eapply is_ctrace_insert with (t' := (trigger EYield ;; k v1)%itree); first done.
     { rewrite /compile_expr. simpl_itree. reflexivity. }
     eapply is_ctrace_yield. { rewrite list_lookup_insert //. by apply lookup_lt_is_Some. }
     by rewrite list_insert_insert.
   - exists (CTYield tid' tr). split; first split; eauto.
-    { intros Hstuck. constructor. by apply Hub. }
+    { apply trace_invariant_postfix_postfix with (tr := tr); eauto. repeat constructor. }
     rewrite compile_expr_val !bind_ret_l in Htr.
     eapply is_ctrace_insert with (t' := (trigger EYield ;; k v2)%itree); first done.
     { rewrite /compile_expr. simpl_itree. reflexivity. }
     eapply is_ctrace_yield. { rewrite list_lookup_insert //. by apply lookup_lt_is_Some. }
     by rewrite list_insert_insert.
   - exists (CTYield tid' tr). split; first split; eauto.
-    { intros Hstuck. constructor. by apply Hub. }
+    { apply trace_invariant_postfix_postfix with (tr := tr); eauto. repeat constructor. }
     eapply is_ctrace_insert; first done.
     { simpl. rewrite /compile_expr. simpl_itree. reflexivity. }
     eapply is_ctrace_yield.
@@ -1003,7 +1120,7 @@ Proof.
     rewrite list_insert_insert.
     by simpl_itree in Htr.
   - exists (CTYield tid' tr). split; first split; eauto.
-    { intros Hstuck. constructor. by apply Hub. }
+    { apply trace_invariant_postfix_postfix with (tr := tr); eauto. repeat constructor. }
     eapply is_ctrace_insert; first done.
     { simpl. rewrite /compile_expr. simpl_itree. reflexivity. }
     eapply is_ctrace_yield.
@@ -1012,7 +1129,7 @@ Proof.
     by simpl_itree in Htr.
   - destruct (AllocN_free_locations _ _ _ _ _ _ Hbase) as [ll <-].
     exists (CTVis state (subevent _ EGetState) σ1 (CTVis (free_locations n σ1) (subevent _ (EDemonic (free_locations n σ1))) ll (CTVis () (subevent _ (ESetState (state_init_heap (`ll) n v σ1))) () (CTYield tid' tr)))). split; first split; eauto.
-    { intros Hstuck. do 4 constructor. by apply Hub. }
+    { apply trace_invariant_postfix_postfix with (tr := tr); eauto. repeat constructor. }
     { simpl. rewrite decide_True //. }
     eapply is_ctrace_insert; first done.
     { simpl. rewrite /compile_expr. simpl_itree. reflexivity. }
@@ -1030,7 +1147,7 @@ Proof.
     rewrite list_insert_insert.
     by simpl_itree in Htr.
   - exists (CTVis state (subevent _ EGetState) σ1 (CTVis () (subevent _ (ESetState (state_upd_heap <[l:=None]> σ1))) () (CTYield tid' tr))). split; first split; eauto.
-    { intros Hstuck. do 3 constructor. by apply Hub. }
+    { apply trace_invariant_postfix_postfix with (tr := tr); eauto. repeat constructor. }
     { simpl. rewrite decide_True //. }
     eapply is_ctrace_insert; first done.
     { simpl. rewrite /compile_expr. simpl_itree. reflexivity. }
@@ -1045,7 +1162,7 @@ Proof.
     rewrite list_insert_insert.
     by simpl_itree in Htr.
   - exists (CTVis state (subevent _ EGetState) σ2 (CTYield tid' tr)). split; first split; eauto.
-    { intros Hstuck. do 2 constructor. by apply Hub. }
+    { apply trace_invariant_postfix_postfix with (tr := tr); eauto. repeat constructor. }
     { simpl. rewrite decide_True //. }
     eapply is_ctrace_insert; first done.
     { simpl. rewrite /compile_expr. simpl_itree. reflexivity. }
@@ -1058,7 +1175,7 @@ Proof.
     rewrite list_insert_insert.
     by simpl_itree in Htr.
   - exists (CTVis state (subevent _ EGetState) σ1 (CTVis () (subevent _ (ESetState (state_upd_heap <[l:=Some w]> σ1))) () (CTYield tid' tr))). split; first split; eauto.
-    { intros Hstuck. do 3 constructor. by apply Hub. }
+    { apply trace_invariant_postfix_postfix with (tr := tr); eauto. repeat constructor. }
     { simpl. rewrite decide_True //. }
     eapply is_ctrace_insert; first done.
     { simpl. rewrite /compile_expr. simpl_itree. reflexivity. }
@@ -1073,7 +1190,7 @@ Proof.
     rewrite list_insert_insert.
     by simpl_itree in Htr.
   - exists (CTVis state (subevent _ EGetState) σ1 (CTVis () (subevent _ (ESetState (state_upd_heap <[l:=Some v2]> σ1))) () (CTYield tid' tr))). split; first split; eauto.
-    { intros Hstuck. do 3 constructor. by apply Hub. }
+    { apply trace_invariant_postfix_postfix with (tr := tr); eauto. repeat constructor. }
     { simpl. rewrite decide_True //. }
     eapply is_ctrace_insert; first done.
     { simpl. rewrite /compile_expr. simpl_itree. reflexivity. }
@@ -1092,7 +1209,7 @@ Proof.
       rewrite bool_decide_eq_true_2 // in Hbase.
       rewrite bool_decide_eq_true_2 // in Htr.
       exists (CTVis state (subevent _ EGetState) σ1 (CTVis () (subevent _ (ESetState (state_upd_heap <[l:=Some v2]> σ1))) () (CTYield tid' tr))). split; first split; eauto.
-      { intros Hstuck. do 3 constructor. by apply Hub. }
+      { apply trace_invariant_postfix_postfix with (tr := tr); eauto. repeat constructor. }
       { simpl. rewrite decide_True //. }
       eapply is_ctrace_insert; first done.
       { simpl. rewrite /compile_expr. simpl_itree. reflexivity. }
@@ -1112,7 +1229,7 @@ Proof.
       rewrite bool_decide_eq_false_2 // in Hbase.
       rewrite bool_decide_eq_false_2 // in Htr.
       exists (CTVis state (subevent _ EGetState) σ1 (CTYield tid' tr)). split; first split; eauto.
-      { intros Hstuck. do 2 constructor. by apply Hub. }
+      { apply trace_invariant_postfix_postfix with (tr := tr); eauto. repeat constructor. }
       { simpl. rewrite decide_True //. }
       eapply is_ctrace_insert; first done.
       { simpl. rewrite /compile_expr. simpl_itree. reflexivity. }
@@ -1125,7 +1242,7 @@ Proof.
       rewrite list_insert_insert.
       by simpl_itree in Htr.
   - exists (CTVis state (subevent _ EGetState) σ1 (CTVis () (subevent _ (ESetState (state_upd_heap <[l:=Some (LitV (LitInt (i1 + i2)))]> σ1))) () (CTYield tid' tr))). split; first split; eauto.
-    { intros Hstuck. do 3 constructor. by apply Hub. }
+    { apply trace_invariant_postfix_postfix with (tr := tr); eauto. repeat constructor. }
     { simpl. rewrite decide_True //. }
     eapply is_ctrace_insert; first done.
     { simpl. rewrite /compile_expr. simpl_itree. reflexivity. }
@@ -1141,7 +1258,7 @@ Proof.
     by simpl_itree in Htr.
   - exists (CTFork (compile_expr e ;; yield_if_not_val e ;; kill_thread) (CTYield tid' tr)).
     split; first split; eauto.
-    { intros Hstuck. repeat constructor. by apply Hub. }
+    { apply trace_invariant_postfix_postfix with (tr := tr); eauto. repeat constructor. }
     rewrite compile_expr_val !bind_ret_l in Htr.
     eapply trace_base_Fork; first apply Htp.
     eapply is_ctrace_yield.
@@ -1160,20 +1277,25 @@ Proof. lia. Qed.
 (* TODO: Idea: make κ = [] *)
 Lemma has_trace n tp σ tp' σ' κ :
   language.nsteps n (tp, σ) κ (tp', σ') →
-  length (compile_tp tp) > 0 →
+  length tp > 0 →
   ∃ tr tid,
     trace_invariant σ tp' σ' tr ∧
-    is_ctrace (R := ()) tr tid (compile_tp tp).
+    is_ctrace (R := val) tr tid (compile_tp tp).
 Proof.
   revert tp σ tp' σ' κ. induction n as [|n IH]; intros tp σ tp' σ' κ Hstep Hne.
-  { destruct (decide (thread_stuck tp σ)) as [(tid&e&Htp&Hstuck)|].
-    * apply stuck_ub with (tp := tp) (tid := tid) in Hstuck as (tr&Hinv&Htr); last done.
-      exists tr, tid. split; last done. inversion Hstep; subst. done.
-    * inversion Hstep; subst.
-      exists CTCut, 0. split; first split.
-      + by intros Hstuck.
-      + done.
-      + apply is_ctrace_CTCut. rewrite map_length. rewrite compile_tp_len in Hne. lia.
+  { destruct (done_or_undone tp) as [[v Hdone]|Hundone].
+    * assert (Hdone' := Hdone).
+      apply is_ctrace_done in Hdone as Htr.
+      apply trace_invariant_done with (σ := σ) in Hdone' as Htinv.
+      exists (CTRet v), 0. inversion Hstep. subst. by split.
+    * destruct (decide (thread_stuck tp σ)) as [(tid&e&Htp&Hstuck)|].
+      + apply stuck_ub with (tp := tp) (tid := tid) in Hstuck as (tr&Hinv&Htr); eauto.
+        exists tr, tid. split; last done. inversion Hstep; subst. done.
+      + inversion Hstep; subst.
+        exists CTCut, 0. split; first split.
+        ++ apply trace_invariant_postfix_undone; first done. by intros Hstuck.
+        ++ done.
+        ++ apply is_ctrace_CTCut. rewrite map_length enumerate_length //.
   }
   inversion Hstep as [|m [tp1 σ1] [tp2 σ2] [tp3 σ3] ? ? Hstep'' Hstep']. subst.
   inversion Hstep'' as [e1' σ1 e2' σ2' efs tpa tpb Htp' Htp2' Hprim].
@@ -1181,53 +1303,76 @@ Proof.
   injection Htp2'. intros -> ->. clear Htp2'.
   inversion Hprim as [K e1 e2 He1 He2 Hbase]. subst. simpl in K, e1, e2.
   clear Hstep'' Hprim.
+  (* TODO: Use [compile_expr_bind'] *)
   destruct (decide (length K = 0)) as [HK|HK].
   - apply nil_length_inv in HK as ->. simpl. simpl in *.
     apply IH in Hstep' as [tr [tid [Hinv Htr]]]; last first.
-    { rewrite compile_tp_len app_length /= app_length.
-      rewrite compile_tp_len app_length /= in Hne.
+    { rewrite app_length /= app_length.
+      rewrite app_length /= in Hne.
       lia.
     }
-    apply step_in_thread with (tp := (compile_tp tpa ++ (v ← compile_expr e1; yield_if_not_val e1;; kill_thread)%itree :: compile_tp tpb)) (tid := length (compile_tp tpa)) (tid' := tid) (k := λ v, kill_thread) (tr := tr) (tp' := tp') (σ' := σ') in Hbase as [tr' [Hinv' Htr']].
-    * exists tr'. exists (length (compile_tp tpa)). rewrite compile_tp_app. eauto.
-    * replace (length (compile_tp tpa)) with (length (compile_tp tpa) + 0) by lia.
-      rewrite compile_tp_app in Htr.
-      rewrite insert_app_r /= -app_assoc /=.
-      by rewrite /= compile_tp_app in Htr.
-    * done.
-    * by apply list_lookup_middle.
+    destruct (decide (length tpa = 0)) as [Htpa|Htpa].
+    * apply nil_length_inv in Htpa as ->. simpl. simpl in *.
+      apply step_in_thread with (tp := ((v ← compile_expr e1; yield_if_not_val e1;; Ret v)%itree :: compile_tp' tpb)) (tid := 0) (tid' := tid) (k := λ v, Ret v) (tr := tr) (tp' := tp') (σ' := σ') in Hbase as [tr' [Hinv' Htr']].
+      + exists tr', 0. rewrite compile_tp_cons //.
+      + simpl. rewrite compile_tp_cons compile_tp'_app // in Htr.
+      + done.
+      + done.
+    * apply step_in_thread with (tp := (compile_tp tpa ++ (v ← compile_expr e1; yield_if_not_val e1;; kill_thread)%itree :: compile_tp' tpb)) (tid := length (compile_tp tpa)) (tid' := tid) (k := λ v, kill_thread) (tr := tr) (tp' := tp') (σ' := σ') in Hbase as [tr' [Hinv' Htr']].
+      + exists tr'. exists (length (compile_tp tpa)). rewrite compile_tp_app //.
+      + replace (length (compile_tp tpa)) with (length (compile_tp tpa) + 0) by lia.
+        rewrite compile_tp_app // in Htr.
+        rewrite insert_app_r /= -app_assoc /=.
+        rewrite compile_tp'_cons compile_tp'_app // in Htr.
+      + done.
+      + by apply list_lookup_middle.
   - apply IH in Hstep' as [tr [tid [Hinv Htr]]]; last first.
     { rewrite -lt_gt -Nat.neq_0_lt_0. intros Hemp%nil_length_inv.
-      rewrite !compile_tp_app /= in Hemp.
       apply app_eq_nil in Hemp as [_ [=]].
     }
-    rewrite compile_tp_app /= compile_tp_app in Htr.
-    rewrite compile_tp_app /=.
-    apply step_in_thread with (tp := (compile_tp tpa ++ (v ← compile_expr e1; yield_if_not_val e1;; compile_expr (fill K (Val v));; trigger EYield;; kill_thread)%itree :: compile_tp tpb)) (tid := length (compile_tp tpa)) (tid' := tid) (k := λ v, (compile_expr (fill K (Val v));; trigger EYield;; kill_thread)%itree) (tr := tr) (tp' := tp') (σ' := σ') in Hbase as [tr' [Hinv' Htr']].
-    * exists tr'. exists (length (compile_tp tpa)).
-      split; first done.
-      rewrite /= compile_expr_bind.
-      + setoid_rewrite fill_not_val; last first. { rewrite -lt_gt -Nat.neq_0_lt_0 //. }
-        rewrite bind_bind. by setoid_rewrite bind_bind.
-      + admit.
-      + rewrite -lt_gt -Nat.neq_0_lt_0 //.
-    * replace (length (compile_tp tpa)) with (length (compile_tp tpa) + 0) by lia.
-      rewrite insert_app_r /= -app_assoc /=.
-      rewrite compile_expr_bind in Htr.
-      + setoid_rewrite fill_not_val in Htr; last first. { rewrite -lt_gt -Nat.neq_0_lt_0 //. }
-        by repeat setoid_rewrite bind_bind in Htr.
-      + admit.
-      + rewrite -lt_gt -Nat.neq_0_lt_0 //.
-    * done.
+    destruct (decide (length tpa = 0)) as [Htpa|Htpa].
+    * apply nil_length_inv in Htpa as ->. simpl. simpl in *.
+      apply step_in_thread with (tp := ((v ← compile_expr e1; yield_if_not_val e1;; w ← compile_expr (fill K (Val v)); trigger EYield;; Ret w)%itree :: compile_tp' tpb)) (tid := 0) (tid' := tid) (k := λ v, (w ← compile_expr (fill K (Val v)); trigger EYield;; Ret w)%itree) (tr := tr) (tp' := tp') (σ' := σ') in Hbase as [tr' [Hinv' Htr']].
+      + exists tr'. exists 0.
+        split; first done.
+        rewrite compile_tp_cons /= compile_expr_bind.
+        ++ setoid_rewrite fill_not_val; last first. { rewrite -lt_gt -Nat.neq_0_lt_0 //. }
+           rewrite bind_bind. by setoid_rewrite bind_bind.
+        ++ admit.
+        ++ rewrite -lt_gt -Nat.neq_0_lt_0 //.
+      + simpl.
+        rewrite compile_tp_cons /= compile_expr_bind in Htr.
+        ++ setoid_rewrite fill_not_val in Htr; last first. { rewrite -lt_gt -Nat.neq_0_lt_0 //. }
+           do 2 setoid_rewrite bind_bind in Htr.
+           by rewrite compile_tp'_app in Htr.
+        ++ admit.
+        ++ rewrite -lt_gt -Nat.neq_0_lt_0 //.
+      + done.
+      + done.
+    * rewrite compile_tp_app // in Htr.
+      rewrite compile_tp_app //.
+      apply step_in_thread with (tp := (compile_tp tpa ++ (v ← compile_expr e1; yield_if_not_val e1;; compile_expr (fill K (Val v));; trigger EYield;; kill_thread)%itree :: compile_tp' tpb)) (tid := length tpa) (tid' := tid) (k := λ v, (compile_expr (fill K (Val v));; trigger EYield;; kill_thread)%itree) (tr := tr) (tp' := tp') (σ' := σ') in Hbase as [tr' [Hinv' Htr']].
+      + exists tr'. exists (length tpa).
+        split; first done.
+        rewrite /= compile_expr_bind.
+        ++ setoid_rewrite fill_not_val; last first. { rewrite -lt_gt -Nat.neq_0_lt_0 //. }
+           rewrite bind_bind. by setoid_rewrite bind_bind.
+        ++ admit.
+        ++ rewrite -lt_gt -Nat.neq_0_lt_0 //.
+      + replace (length tpa) with (length (compile_tp tpa) + 0) by rewrite compile_tp_len //.
+        rewrite insert_app_r /= -app_assoc /=.
+        rewrite compile_tp'_cons compile_tp'_app /= compile_expr_bind in Htr.
+        ++ setoid_rewrite fill_not_val in Htr; last first. { rewrite -lt_gt -Nat.neq_0_lt_0 //. }
+           by repeat setoid_rewrite bind_bind in Htr.
+        ++ admit.
+        ++ rewrite -lt_gt -Nat.neq_0_lt_0 //.
+      + done.
 Admitted.
 
-Definition trace_ends_in_ub {E R} `{ubE -< E} (tr : trace E R) :=
-  is_postfix (TVisEmpty void (subevent _ EUb)) tr.
-
 Lemma interp_tr_state_ub {E R S} `{EqDecision S} `{ubE -< E} σ (tr : trace (stateE S +' E) R) tr' :
-  trace_ends_in_ub tr →
+  trace_terminates_in tr TermUb →
   interp_tr_state σ tr = Some tr' →
-  trace_ends_in_ub tr'.
+  trace_terminates_in tr' TermUb.
 Proof.
   revert σ tr'. induction tr; intros σ tr' Hub Hst.
   - inversion Hub.
@@ -1244,58 +1389,75 @@ Proof.
   - inversion Hub.
 Qed.
 
-Lemma interp_tr_ub {E E' R} `{ubE -< E'} (tr : trace (E +' E') R) :
-  trace_ends_in_ub tr →
-  trace_ends_in_ub (interp_tr tr).
+Lemma interp_tr_term {E E' R} `{ubE -< E'} (tr : trace (E +' E') R) (tx : Terminal R) :
+  trace_terminates_in tr tx →
+  trace_terminates_in (interp_tr tr) tx.
+Admitted.
+
+Lemma sequencify_term {E E' R} `{ubE -< E'} (tr : ctrace (E +' E') R) (tx : Terminal R) :
+  ctrace_terminates_in tr tx →
+  trace_terminates_in (sequencify tr) (inl <$> tx).
+Admitted.
+
+Lemma interp_tr_state_ret {E R S} `{EqDecision S} `{ubE -< E} σ (tr : trace (stateE S +' E) R) tr' (r : R) :
+  trace_terminates_in tr (TermRet r) →
+  interp_tr_state σ tr = Some tr' →
+  ∃ σ, trace_terminates_in tr' (TermRet (σ, r)).
 Proof.
-  intros Hub.
-  rewrite /trace_ends_in_ub.
-  replace (TVisEmpty void (subevent void EUb))
-    with (interp_tr (R := R) (TVisEmpty void (subevent void EUb : (E +' E') void)))
-    by done.
-  by apply interp_tr_is_postfix.
+  revert σ tr'. induction tr; intros σ tr' Hret Hst.
+  - inversion Hret. injection Hst as <-. exists σ. constructor.
+  - destruct e as [e|e]; first destruct e as [|σ'].
+    * simpl in Hst. destruct (decide (a = σ)) as [->|]; last discriminate.
+      apply IHtr with (σ := σ); last done. by inversion Hret.
+    * inversion Hret; simplify_K; simplify_K; subst. by eapply IHtr.
+    * simpl in Hst. destruct (interp_tr_state σ tr) as [tr''|] eqn:Heq.
+      + simpl in Heq. injection Hst as <-.
+        inversion Hret. subst. simplify_K.
+        apply IHtr in Heq as [σ' Hterm]; last done.
+        exists σ'. by constructor.
+      + discriminate.
+  - inversion Hret; simplify_K; simplify_K; subst.
+  - inversion Hret.
 Qed.
 
-Lemma sequencify_ub {E E' R} `{ubE -< E'} (tr : ctrace (E +' E') R) :
-  is_postfix_ctrace (CTVisEmpty void (subevent _ EUb)) tr →
-  trace_ends_in_ub (sequencify tr).
-Proof.
-  intros Hub.
-  rewrite /trace_ends_in_ub.
-  replace (TVisEmpty void (subevent void EUb))
-    with (sequencify (R := R) (CTVisEmpty void (subevent void EUb : (E +' E') void)))
-    by done.
-  by apply sequencify_is_postfix.
-Qed.
-
-Lemma is_trace_ub {R} (t : itree ubE R) tr :
-  trace_ends_in_ub tr →
+Lemma is_trace_term {R} (t : itree ubE R) tr tx :
+  trace_terminates_in tr tx →
   is_trace tr t →
-  t ≈ ub.
+  t ≈ match tx with
+      | TermUb => ub
+      | TermRet r => Ret r
+      end.
+Admitted.
+(*
 Proof.
-  intros Hub Htr. pfold. rewrite /eqit_. induction Htr.
+  intros Hterm Htr. pfold. rewrite /eqit_. induction Htr.
   - inversion Hub.
   - by destruct e.
   - inversion Hub. destruct e. constructor. by intros.
   - inversion Hub.
   - constructor; first done. by apply IHHtr.
 Qed.
+*)
 
-Lemma ub_execution n e σ tp' σ' κ :
+Lemma execution n e σ tp' σ' κ tx :
   language.nsteps n ([e], σ) κ (tp', σ') →
-  thread_stuck tp' σ' →
+  tp_termination tp' σ' = Some tx →
   ∃ t1 t2 t3,
     (* TODO: consisting naming for interpretion relations *)
     (* TODO: abstraction for this composite relation *)
-    interleaves (R := ()) 0 [compile_expr e ;; yield_if_not_val e ;; kill_thread]%itree t1 ∧
+    interleaves (R := val) 0 [v ← compile_expr e ; yield_if_not_val e ;; Ret v]%itree t1 ∧
     demonic_instantiates t1 t2 ∧
     eval σ t2 t3 ∧
     (* TODO: use UB adequacy *)
-    t3 ≈ ub.
+    match tx with
+    | TermUb => t3 ≈ ub
+    | TermRet r => ∃ σ', t3 ≈ Ret (σ', inl r)
+    end.
 Proof.
-  intros Hsteps Hstuck.
-  apply has_trace in Hsteps as (tr&tid&[Hub [tr' Hst]]&Htr); last eauto.
-  apply Hub in Hstuck as Hub'.
+  intros Hsteps Hterm.
+  apply has_trace in Hsteps as (tr&tid&[Htinv [tr' Hst]]&Htr); last eauto.
+  rewrite /trace_invariant_postfix in Htinv.
+  rewrite Hterm in Htinv.
   apply interleaving_extending_trace in Htr as (t1&Hint&Htr).
   exists t1.
   eapply instantiation_extending_trace in Htr as (t2&Hinst&Htr).
@@ -1308,36 +1470,48 @@ Proof.
   }
   split; first done.
   split; first done.
-  eapply is_trace_ub; last done.
-  eapply interp_tr_state_ub; last done. apply interp_tr_ub. by apply sequencify_ub.
+  destruct tx.
+  - apply sequencify_term in Htinv. apply interp_tr_term in Htinv.
+    eapply interp_tr_state_ret in Htinv as [σ'' Htinv]; last done.
+    exists σ''. by apply is_trace_term with (t := t3) (tr := tr') (tx := TermRet (σ'', inl r)).
+  - apply is_trace_term with (t := t3) (tr := tr') (tx := TermUb); last done.
+    eapply interp_tr_state_ub; last done. apply interp_tr_term. by apply sequencify_term in Htinv.
 Qed.
 
-Lemma ub_execution_wpi' `{!invGS_gen hlc Σ} n e σ tp' σ' κ :
+Lemma execution_wpi' `{!invGS_gen hlc Σ} n e σ tp' σ' κ tx Φ :
   language.nsteps n ([e], σ) κ (tp', σ') →
-  thread_stuck tp' σ' →
+  tp_termination tp' σ' = Some tx →
   state_interp σ -∗
-  WPi (compile_expr e;; yield_if_not_val e;; kill_thread : itree heaplangE ()) @ heaplangH ; ⊤ {{ _, True }} -∗
-  |={⊤}=> False.
+  WPi (v ← compile_expr e; yield_if_not_val e;; Ret v) @ heaplangH ; ⊤ {{ Φ }} -∗
+  |={⊤}=> match tx with
+  | TermUb => False
+  | TermRet v => Φ v
+  end.
 Proof.
   iIntros (Hstep Hstuck) "Hstate Hwp".
-  apply ub_execution in Hstep as (t1&t2&t3&Hint&Hinst&Heval&Hub); last done.
+  apply execution with (tx := tx) in Hstep as (t1&t2&t3&Hint&Hinst&Heval&Hterm); last done.
   (* TODO: Name these adequacy theorems consistently. *)
   iDestruct (threadpool_adequacy with "Hwp") as "Hwp"; first apply Hint.
   iDestruct (demonicH_adequate with "Hwp") as "Hwp"; first apply Hinst.
   iDestruct (wpi_state with "Hstate Hwp") as "Hwp"; first apply Heval.
-  rewrite Hub /ub -wpi_vis' /=. by iMod "Hwp".
+  destruct tx.
+  - destruct Hterm as [σ'' Hterm]. rewrite Hterm -wpi_ret'. by iMod "Hwp" as "[_ HΦ]".
+  - rewrite Hterm /ub -wpi_vis' /=. by iMod "Hwp".
 Qed.
 
-Lemma ub_execution_wpi `{!invGS_gen hlc Σ} n e σ tp' σ' κ :
+Lemma ub_execution_wpi `{!invGS_gen hlc Σ} n e σ tp' σ' κ tx Φ :
   language.nsteps n ([e], σ) κ (tp', σ') →
-  thread_stuck tp' σ' →
+  tp_termination tp' σ' = Some tx →
   state_interp σ -∗
-  WPi (compile_expr e) @ heaplangH ; ⊤ {{ _, True }} -∗
-  |={⊤}=> False.
+  WPi (compile_expr e) @ heaplangH ; ⊤ {{ Φ }} -∗
+  |={⊤}=> match tx with
+  | TermUb => False
+  | TermRet v => Φ v
+  end.
 Proof.
-  iIntros (Hstep Hstuck) "Hstate Hwp".
-  iApply (ub_execution_wpi' with "Hstate"); eauto.
+  iIntros (Hstep Hterm) "Hstate Hwp".
+  iApply (execution_wpi' with "Hstate"); eauto.
   iApply wpi_bind. iApply wpi_wand; last done.
-  iIntros (r) "_". iApply wpi_bind. iApply @wpi_yield_if_not_val.
-  iApply @wpi_kill.
+  iIntros (r) "HΦ". iApply wpi_bind. iApply @wpi_yield_if_not_val.
+  by iApply @wpi_ret.
 Qed.
